concurrency/hack-hash-table-wrap/MapSpec.s.dfy
@@ -1,0 +1,117 @@
+include "../../lib/Lang/NativeTypes.s.dfy"
+
+module KeyValueType {
+  import opened NativeTypes
+
+  type Key = uint64
+  type Value(==)
+
+  datatype QueryResult = Found(val: Value) | NotFound
+}
+
+module InputOutputIfc {
+  type Input(!new)
+  type Output(!new)
+
+  datatype Op = Op(input: Input, output: Output)
+}
+
+module MapIfc refines InputOutputIfc {
+  import opened KeyValueType
+
+  datatype Input =
+    | QueryInput(key: Key)
+    | InsertInput(key: Key, value: Value)
+
+  datatype Output =
+    | QueryOutput(res: QueryResult)
+    | InsertOutput
+}
+
+module AsyncIfc {
+  import Ifc = MapIfc
+  type {:extern} RequestId(==,!new)
+
+  datatype Op =
+    | Start(rid: RequestId, input: Ifc.Input)
+    | End(rid: RequestId, output: Ifc.Output)
+    | InternalOp
+}
+
+// disallowed:
+
+module MapSpec {
+  import opened KeyValueType
+
+  import Ifc = MapIfc
+  datatype Variables = Variables(m: map<Key, Value>)
+
+  predicate Init(s: Variables) {
+    s.m == map[]
+  }
+
+  predicate Next(s: Variables, s': Variables, op: Ifc.Op) {
+    match op {
+      case Op(input, output) => (
+        match input {
+          case QueryInput(key) => 
+            && s' == s
+            && (key in s.m ==> output == Ifc.QueryOutput(Found(s.m[key])))
+            && (key !in s.m ==> output == Ifc.QueryOutput(NotFound))
+          case InsertInput(key, value) =>
+            && s'.m == s.m[key := value]
+            && output == Ifc.InsertOutput
+        }
+      )
+    }
+  }
+}
+
+module AsyncSpec {
+  import InnerIfc = MapIfc
+  import SM = MapSpec
+  import Ifc = AsyncIfc
+
+  type RequestId = Ifc.RequestId
+
+  datatype Req = Req(rid: RequestId, input: InnerIfc.Input)
+  datatype Resp = Resp(rid: RequestId, output: InnerIfc.Output)
+
+  datatype Variables = Variables(
+      s: SM.Variables,
+      reqs: multiset<Req>,
+      resps: multiset<Resp>)
+
+  predicate Init(s: Variables)
+  {
+    && SM.Init(s.s)
+    && s.reqs == multiset{}
+    && s.resps == multiset{}
+  }
+
+  predicate Next(s: Variables, s': Variables, op: Ifc.Op)
+  {
+    match op {
+      case Start(rid, input) =>
+        // add 'input' to 'reqs'
+        && s' == s.(reqs := s.reqs + multiset{Req(rid, input)})
+      case InternalOp => (
+        // stutter step
+        || (s' == s)
+        // resolve request step
+        // serialization point: remove 'input' from 'reqs',
+        // add 'output' to 'resps'
+        || (exists rid, input, output ::
+          && Req(rid, input) in s.reqs
+          && s'.reqs == s.reqs - multiset{Req(rid, input)}
+          && s'.resps == s.resps + multiset{Resp(rid, output)}
+          && SM.Next(s.s, s'.s, InnerIfc.Op(input, output))
+        )
+      )
+      case End(rid, output) =>
+        // remove from 'resps'
+        && Resp(rid, output) in s.resps
+        && s' == s.(resps := s'.resps - multiset{Resp(rid, output)})
+    }
+  }
+}
