concurrency/hack-hash-table-wrap/RobinHood.i.dfy
@@ -1,0 +1,559 @@
+include "MapSpec.s.dfy"
+include "../../lib/Base/Option.s.dfy"
+
+module RobinHood {
+  import opened KeyValueType
+  import opened NativeTypes
+  import opened Options
+
+
+  function method hash(key: uint64) : (h : uint32)
+
+  datatype Entry =
+    | Full(key: Key, value: Value)
+    | Empty
+
+  predicate KeysUnique(table: seq<Entry>)
+  {
+    forall i, j | 0 <= i < |table| && 0 <= j < |table|
+        && i != j && table[i].Full? && table[j].Full?
+        :: table[i].key != table[j].key
+  }
+
+  /*predicate ValidHashEntry(table: seq<Entry>, i: int, j: int)
+  requires 0 <= i < |table|
+  requires 0 <= j < |table|
+  {
+    table[i].Empty? && table[j].Full? ==> (
+      var h := hash(table[j].key)
+      // we need h to be between i and j, but cyclically
+      && (i < j ==> i < h <= j)
+      && (i > j ==> i < h || h <= j)
+    )
+  }*/
+
+  /*predicate ValidHashNeighbors(table: seq<Entry>, i: int, j: int)
+  requires 0 <= i < |table|
+  requires 0 <= j < |table|
+  {
+    var k := (if j+1 < |table| then j+1 else 0);
+    table[i].Empty? && table[j].Full? && table[j+1].Full? ==> (
+      var h := hash(table[j].key)
+      // we need h to be between i and j, but cyclically
+      && (i < j ==> i < h <= j)
+      && (i > j ==> i < h || h <= j)
+    )
+  }*/
+
+  predicate ContiguousToEntry(table: seq<Entry>, i: int)
+  requires 0 <= i < |table|
+  {
+    table[i].Full? ==> (
+      var h := hash(table[i].key) as int;
+      && (h <= i ==> (forall j | h <= j <= i :: table[j].Full?))
+      && (h > i ==>
+        && h < |table|
+        && (forall j | 0 <= j <= i :: table[j].Full?)
+        && (forall j | h <= j < |table| :: table[j].Full?)
+      )
+    )
+  }
+
+  // 'Robin Hood' order
+  // It's not enough to say that hash(entry[i]) <= hash(entry[i+1])
+  // because of wraparound. We do a cyclic comparison 'rooted' at an
+  // arbitrary empty element, given by e.
+  predicate ValidHashNeighbors(table: seq<Entry>, e: int, j: int)
+  requires 0 <= e < |table|
+  requires 0 <= j < |table|
+  {
+    var k := (if j+1 < |table| then j+1 else 0);
+    (table[e].Empty? && table[j].Full? && table[k].Full? ==> (
+      var hj := hash(table[j].key) as int;
+      var hk := hash(table[k].key) as int;
+      (e < hj <= hk || hj <= hk < e || hk < e < hj)
+    ))
+  }
+
+  predicate ExistsEmptyEntry(table: seq<Entry>)
+  {
+    exists i :: 0 <= i < |table| && table[i].Empty?
+  }
+
+  predicate Inv(table: seq<Entry>)
+  {
+    && KeysUnique(table)
+    && ExistsEmptyEntry(table)
+    && (forall e, j | 0 <= e < |table| && 0 <= j < |table|
+        :: ValidHashNeighbors(table, e, j))
+    && (forall i | 0 <= i < |table|
+        :: ContiguousToEntry(table, i))
+  }
+
+  // Ops
+
+  // Map interpretation, queries
+
+  function GetIndex(table: seq<Entry>, key: Key) : Option<int>
+  {
+    if i :| 0 <= i < |table| && table[i].Full? && table[i].key == key then (
+      Some(i)
+    ) else (
+      None
+    )
+  }
+
+  function GetValue(table: seq<Entry>, key: Key) : Option<Value>
+  {
+    var i := GetIndex(table, key);
+    if i.Some? then Some(table[i.value].value) else None
+  }
+
+  lemma GetValue_for_found(table: seq<Entry>, i: int)
+  requires Inv(table)
+  requires 0 < i < |table|
+  requires table[i].Full?
+  ensures GetValue(table, table[i].key) == Some(table[i].value)
+  {
+  }
+
+  predicate NotFoundInRange(table: seq<Entry>, key: Key, i: int)
+  {
+    var h := hash(key) as int;
+    && 0 < i < |table|
+    && table[i].Empty? // TODO could also use a comparison condition on the hash value
+    && (h <= i ==> (forall j | h <= j < i :: table[j].Full? && table[j].key != key))
+    && (h > i ==> (forall j | 0 <= j < i :: table[j].Full? && table[j].key != key))
+    && (h > i ==> (forall j | h <= j < |table| :: table[j].Full? && table[j].key != key))
+  }
+
+  lemma GetValue_for_not_found(table: seq<Entry>, key: Key, i: int)
+  requires Inv(table)
+  requires NotFoundInRange(table, key,i)
+  ensures GetValue(table, key) == None
+  {
+    forall j | 0 <= j < |table| && table[j].Full? && table[j].key == key
+    ensures false
+    {
+      assert ContiguousToEntry(table, j);
+      /*var h := hash(key) as int;
+      if h <= j {
+        if j < i {
+          assert false;
+        } else {
+          assert false;
+        }
+      } else {
+        assert false;
+      }*/
+    }
+  }
+
+  // Update existing key
+
+  predicate Update(table: seq<Entry>, table': seq<Entry>, i: int, key: Key, value: Value)
+  {
+    && 0 <= i < |table|
+    && table[i].Full?
+    && table[i].key == key
+    && table' == table[i := Full(key, value)]
+  }
+
+  lemma Update_Inv(table: seq<Entry>, table': seq<Entry>, i: int, key: Key, value: Value)
+  requires Inv(table)
+  requires Update(table, table', i, key, value)
+  ensures Inv(table')
+  {
+    var i :| 0 <= i < |table| && table[i].Empty?;
+    assert table'[i].Empty?;
+
+    forall e, j | 0 <= e < |table'| && 0 <= j < |table'|
+    ensures ValidHashNeighbors(table', e, j)
+    {
+      assert ValidHashNeighbors(table, e, j);
+    }
+
+    forall i | 0 <= i < |table'|
+    ensures ContiguousToEntry(table', i)
+    {
+      assert ContiguousToEntry(table, i);
+    }
+  }
+
+  lemma GetValue_Update_self(
+      table: seq<Entry>, table': seq<Entry>,
+      i: int, key: Key, value: Value)
+  requires Inv(table)
+  requires Update(table, table', i, key, value)
+  ensures GetValue(table', key) == Some(value)
+  {
+    assert table'[i].key == key; // observe
+    //assert GetIndex(table', key) == Some(i);
+  }
+
+  lemma GetValue_Update_other(
+      table: seq<Entry>, table': seq<Entry>,
+      i: int, key: Key, value: Value, other: Key)
+  requires Inv(table)
+  requires Update(table, table', i, key, value)
+  requires other != key
+  ensures GetValue(table', other) == GetValue(table, other)
+  {
+    if GetIndex(table, other).Some? {
+      var j := GetIndex(table, other).value;
+      assert table'[j].key == other;
+      //assert GetIndex(table', other) == Some(j);
+      //assert GetIndex(table, other) == GetIndex(table', other);
+      //assert j != i;
+    } else if GetIndex(table', other).Some? {
+      //assert GetIndex(table, other) == GetIndex(table', other);
+    } else {
+      //assert GetIndex(table, other) == GetIndex(table', other);
+    }
+  }
+
+  // Remove a key
+
+  // delete a, then shift a+1,...,b to the left
+  datatype LeftShift = LeftShift(start: int, end: int)
+
+  predicate ApplyLeftShift(table: seq<Entry>, table': seq<Entry>, shift: LeftShift)
+  {
+    && 0 <= shift.start < |table|
+    && 0 <= shift.end < |table|
+    && |table'| == |table|
+
+    && (shift.start <= shift.end ==>
+      && (forall i | 0 <= i < shift.start :: table'[i] == table[i])
+      && (forall i | shift.start <= i < shift.end :: table'[i] == table[i+1])
+      && table'[shift.end] == Empty
+      && (forall i | shift.end < i < |table'| :: table'[i] == table[i])
+    )
+
+    && (shift.start > shift.end ==>
+      && (forall i | 0 <= i < shift.end :: table'[i] == table[i+1])
+      && table'[shift.end] == Empty
+      && (forall i | shift.end < i < shift.start :: table'[i] == table[i])
+      && (forall i | shift.start <= i < |table'| - 1 :: table'[i] == table[i+1])
+      && table'[|table'| - 1] == table[0]
+    )
+  }
+
+  predicate Remove(table: seq<Entry>, table': seq<Entry>, key: Key, shift: LeftShift)
+  {
+    && 0 <= shift.start < |table|
+    && 0 <= shift.end < |table|
+    && table[shift.start].Full?
+    && table[shift.start].key == key
+
+    // The next element after 'end' should be the first element which is either
+    // (i) empty or (ii) has hash value equal to its slot index
+    && var next := (if shift.end == |table| - 1 then 0 else shift.end + 1);
+    && (table[next].Full? ==> hash(table[next].key) as int == next)
+    && (shift.start <= shift.end ==> forall j | shift.start < j <= shift.end
+            :: table[j].Full? && hash(table[j].key) as int != j)
+    && (shift.end < shift.start ==> forall j | (shift.start < j < |table| || 0 <= j <= shift.end)
+            :: table[j].Full? && hash(table[j].key) as int != j)
+
+    && ApplyLeftShift(table, table', shift)
+  }
+
+  predicate AllBetweenAreFull(table: seq<Entry>, a: int, b: int)
+  {
+    && 0 <= a < |table|
+    && 0 <= b < |table|
+    && (a < b ==> forall k | a < k < b :: table[k].Full?)
+    && (a > b ==> forall k | 0 <= k < b :: table[k].Full?)
+    && (a > b ==> forall k | a < k < |table| :: table[k].Full?)
+  }
+
+  lemma get_empty_slot_backwards(table: seq<Entry>, i: int)
+  returns (j: int)
+  requires 0 <= i < |table|
+  requires ExistsEmptyEntry(table)
+  ensures 0 <= j < |table|
+  ensures table[j].Empty?
+  ensures AllBetweenAreFull(table, j, i)
+  {
+    if table[i].Empty? {
+      j := i;
+      return;
+    }
+
+    j := i;
+    while table[j].Full?
+    invariant 0 <= j < |table|
+    invariant AllBetweenAreFull(table, j, i)
+    decreases |table| - (if j <= i then i - j else i - j + |table|)
+    {
+      if j == i+1 {
+        assert false;
+      }
+      j := if j == 0 then |table| - 1 else j - 1;
+    }
+  }
+
+  lemma get_empty_slot_forwards(table: seq<Entry>, i: int)
+  returns (j: int)
+  requires 0 <= i < |table|
+  requires ExistsEmptyEntry(table)
+  ensures 0 <= j < |table|
+  ensures table[j].Empty?
+  ensures AllBetweenAreFull(table, i, j)
+  {
+    if table[i].Empty? {
+      j := i;
+      return;
+    }
+
+    j := i;
+    while table[j].Full?
+    invariant 0 <= j < |table|
+    invariant AllBetweenAreFull(table, i, j)
+    decreases |table| - (if i <= j then j - i else j - i + |table|)
+    {
+      if j == i-1 {
+        assert false;
+      }
+      j := if j == |table| - 1 then 0 else j + 1;
+    }
+  }
+
+  lemma hash_neighbor_transitive(table: seq<Entry>, e: int, i: int, j: int)
+  requires 0 <= e < |table|
+  requires 0 <= i < |table|
+  requires 0 <= j < |table|
+  requires table[e].Empty?
+  requires table[i].Full?
+  requires table[j].Full?
+  requires AllBetweenAreFull(table, i, j)
+  requires (forall j | 0 <= j < |table|
+        :: ValidHashNeighbors(table, e, j))
+  requires (forall i | 0 <= i < |table|
+        :: ContiguousToEntry(table, i))
+  ensures 
+      var hi := hash(table[i].key) as int;
+      var hj := hash(table[j].key) as int;
+      e < hi <= hj || hi <= hj < e || hj < e < hi
+
+  decreases if j >= i then j - i else j - i + |table|
+  {
+    if i == j {
+      assert ContiguousToEntry(table, i);
+      return;
+    }
+
+    assert ValidHashNeighbors(table, e, i);
+
+    var ip := (if i < |table| - 1 then i + 1 else 0);
+    if ip == j {
+      var hi := hash(table[i].key) as int;
+      var hj := hash(table[j].key) as int;
+      assert e != hi;
+      assert e != hj;
+    } else {
+      hash_neighbor_transitive(table, e, ip, j);
+    }
+  }
+
+  lemma Remove_Inv(table: seq<Entry>, table': seq<Entry>, key: Key, shift: LeftShift)
+  requires Inv(table)
+  requires Remove(table, table', key, shift)
+  ensures Inv(table')
+  {
+    forall e, j | 0 <= e < |table| && 0 <= j < |table|
+    ensures ValidHashNeighbors(table', e, j)
+    {
+      /*var e1 :| 0 <= e1 < |table| && table[e1].Empty?;
+      assert table'[e1].Empty?;
+
+      assert ValidHashNeighbors(table', e1, j);
+      assert ValidHashNeighbors(table', e, j);*/
+
+      /*assert ValidHashNeighbors(table, e, j);
+      if e == shift.end {
+        assert ValidHashNeighbors(table', e, j);
+      } else {
+        assert ValidHashNeighbors(table', e, j);
+      }*/
+
+      if e == shift.end {
+        if table'[j].Full? {
+          // suppose X is removed and bbbb is shifted:
+          //
+          // _aaaaXbbbbcccc_
+          // _aaaabbbb_cccc_
+          //
+          // e1       e    e2
+          //
+          // There are four cases for j ... it could be the aaaa, bbbb, cccc, or
+          // somewhere else. 
+          // 
+          // First we find e1 or e2, then determine where j is w.r.t. e1, e, e2
+
+          var e1 := get_empty_slot_backwards(table, e);
+          var e2 := get_empty_slot_forwards(table, e);
+          var e_next := (if e < |table| - 1 then e + 1 else 0);
+
+          //assert !table[e1].Full?;
+          //assert table[shift.start].Full?;
+          //assert e1 < shift.start <= e
+          //    || e < e1 < shift.start
+          //    || shift.start <= e < e1;
+          assert e1 < e < e2
+              || e < e2 <= e1
+              || e2 <= e1 < e;
+
+          if (e < j < e2) || (j < e2 < e) || (e2 < e < j) {
+            // the cccc's case
+            // we have hash(j) <= hash(j+1) w.r.t. position e1
+            assert ValidHashNeighbors(table, e1, j);
+            // we need to get the same w.r.t. position e
+            // so we get e < e + 1 <= e_next == hash(e_next) <= hash(j) w.r.t. e1
+
+            //assert table[j].key == table'[j].key;
+            //assert hash(table[j].key) == hash(table'[j].key);
+            hash_neighbor_transitive(table, e1, e_next, j);
+            //assert e1 < e < hash(table[j].key) as int
+            //    || e < hash(table[j].key) as int < e1
+            //    || hash(table[j].key) as int < e1 < e;
+            assert ValidHashNeighbors(table', e, j);
+          } else if (e1 < j < e) || (j < e < e1) || (e < e1 < j) {
+            var k := (if j < |table| - 1 then j + 1 else 0);
+            var l := (if k < |table| - 1 then k + 1 else 0);
+
+            //assert ValidHashNeighbors(table, e1, j);
+            //hash_neighbor_transitive(table, e1, j, e);
+            //assert ValidHashNeighbors(table, e1, k);
+            //hash_neighbor_transitive(table, e1, k, e);
+            //assert ValidHashNeighbors(table, e, j);
+            //assert ValidHashNeighbors(table, e, k);
+            //assert ValidHashNeighbors(table, e2, j);
+            //assert ValidHashNeighbors(table, e2, k);
+            //assert ContiguousToEntry(table, j);
+            assert ContiguousToEntry(table, k);
+            //assert ValidHashNeighbors(table, e2, j);
+            //hash_neighbor_transitive(table, e2, j, e);
+            //assert ValidHashNeighbors(table, e2, k);
+            //hash_neighbor_transitive(table, e2, k, e);
+            //assert ValidHashNeighbors(table, e1, k);
+
+            // aaaa or bbbb case
+            // we have hash(j) <= hash(j+1) w.r.t. position e1
+            assert ValidHashNeighbors(table, e1, j);
+
+            assert ValidHashNeighbors(table, e1, k);
+            hash_neighbor_transitive(table, e1, k, e);
+
+            assert ValidHashNeighbors(table, e1, l);
+            if table[k].Full? && table[l].Full? && l != e && k != e {
+              hash_neighbor_transitive(table, e1, l, e);
+            }
+            // we need to get the same w.r.t. position e
+            // therefore we want
+            // hash(j+1) <= e     w.r.t. position e1
+
+            assert ContiguousToEntry(table, e);
+
+            assert ValidHashNeighbors(table', e, j);
+          } else {
+            assert ValidHashNeighbors(table, e1, j);
+            assert ValidHashNeighbors(table, e2, j);
+
+            //assert ValidHashNeighbors(table', e1, j);
+            //assert ValidHashNeighbors(table', e2, j);
+
+            //assert e2 < j < e1 || j < e1 <= e2 || e1 <= e2 < j;
+
+            /*var k := (if j+1 < |table| then j+1 else 0);
+            if table[j].Full? && table[k].Full? {
+              assert table[j] == table'[j];
+              assert table[k] == table'[k];
+
+              var hj := hash(table[j].key) as int;
+              var hk := hash(table[k].key) as int;
+
+              assert (e1 < hk ==> e1 < hj <= hk);
+              assert (e1 > hk ==> e1 < hj || hj <= hk);
+
+              assert (e2 < hk ==> e2 < hj <= hk);
+              assert (e2 > hk ==> e2 < hj || hj <= hk);
+
+              assert ContiguousToEntry(table, j);
+
+              assert (e < hk ==> e < hj <= hk);
+              assert (e > hk ==> e < hj || hj <= hk);
+            }*/
+
+            assert ContiguousToEntry(table, j);
+
+            assert ValidHashNeighbors(table', e, j);
+          }
+        }
+
+        assert ValidHashNeighbors(table', e, j);
+      } else {
+        // These 3 should handle all the cases. We need j+1 for the case
+        // that slot j+1 shifted left to slot j. And of course we need 0
+        // for the wraparound shift case. We'll let Dafny bash out all the cases.
+        assert ValidHashNeighbors(table, e, j);
+        assert ValidHashNeighbors(table, e, 0);
+        if j+1 < |table| {
+          assert ValidHashNeighbors(table, e, j+1);
+        }
+
+        assert ValidHashNeighbors(table', e, j);
+      }
+    }
+
+    forall i | 0 <= i < |table|
+    ensures ContiguousToEntry(table', i)
+    {
+      if table[i].Full? {
+        assert ContiguousToEntry(table, i);
+        if i < |table| - 1 {
+          assert ContiguousToEntry(table, i+1);
+        } else {
+          assert ContiguousToEntry(table, 0);
+        }
+
+        var e := shift.end;
+        var e1 := get_empty_slot_backwards(table, e);
+        var e2 := get_empty_slot_forwards(table, shift.end);
+
+        var e_next := (if e < |table| - 1 then e + 1 else 0);
+
+        if e < i < e2 || i < e2 < e || e2 < e < i {
+          hash_neighbor_transitive(table, e2, e_next, i);
+          assert ContiguousToEntry(table', i);
+        } else if (shift.start <= i < e) || (i < e < shift.start) || (e < shift.start <= i) {
+          var h := hash(table'[i].key) as int;
+          //var ip := (if i < |table| - 1 then i+1 else 0);
+          //assert h == hash(table[ip].key) as int;
+          assert 0 <= h <= |table| - 1;
+          /*assert e1 < h <= ip || h <= ip < e1 || ip < e1 < h;
+          assert h != ip;
+          assert e1 < h < ip || h < ip < e1 || ip < e1 < h;
+          assert e1 < h <= i || h <= i < e1 || i < e1 < h by {
+            if e1 < h <= ip {
+              assert e1 < h <= i;
+            } else if h <= ip < e1 {
+              assert h <= i < e1;
+            } else if ip < e1 < h {
+              if i == |table| - 1 {
+                assert e1 < h <= i;
+              } else {
+                assert i < e1 < h;
+              }
+            }
+          }*/
+
+          assert ContiguousToEntry(table', i);
+        } else {
+          assert ContiguousToEntry(table', i);
+        }
+      }
+    }
+  }
+
+}
